feat: subject reduction

Cube/Simple.lean
@@ -1,49 +1,70 @@
 import Lean
+import Std.Data.List.Lemmas
+import Mathlib.Init.Algebra.Order
+import Mathlib.Init.Data.Nat.Lemmas
+import Mathlib.Tactic.Linarith
+
 open Lean
 
 namespace List
 
-def findIdx? (p : α → Bool) : List α → Option Nat
-  | []    => none
-  | a::as => match p a with
-    | true  => some 0
-    | false => Nat.succ <*> findIdx? p as
-
-theorem findIdx?_bounds (h : findIdx? p xs = some idx) : idx < xs.length := by
-  induction xs generalizing idx with
+theorem findIdx?_lower_bound (h : findIdx? p xs s = some idx) : s ≤ idx := by
+  induction xs generalizing s with
   | nil => contradiction
   | cons x xs ih =>
-    simp only [findIdx?] at h
+    unfold findIdx? at h
     split at h
-    case cons.h_1 =>
-      injection (Eq.symm h)
-      simp_all_arith
-    case cons.h_2 =>
-      simp only [Seq.seq, Option.bind, (· <$> ·), Option.map] at h
-      split at h
-      case h_1 h2 =>
-        injection (Eq.symm h)
-        simp_all_arith
-      case h_2 => contradiction
+    next => injections; simp_all_arith
+    next =>
+      apply Nat.le_trans
+      next => exact Nat.le_succ s
+      next => simp_all [ih]
 
-theorem findIdx?_prop (h : findIdx? p xs = some idx) : p (getElem xs idx (findIdx?_bounds h)) := by
-  induction xs generalizing idx with
+theorem findIdx?_bounds' (h : findIdx? p xs s = some idx) : idx < xs.length + s := by
+  induction xs generalizing s with
   | nil => contradiction
   | cons x xs ih =>
-    simp only [findIdx?] at h
-    -- For some reason split doesnt work here: TODO Report bug
-    cases h2 : (p x) with
-    | true =>
-      simp[h2] at h
-      have h3 := Eq.symm h
-      simp[GetElem.getElem, h3, List.get, h2]
-    | false =>
-      simp only [Seq.seq, Option.bind, (· <$> ·), Option.map, h2] at h
-      split at h
-      case cons.false.h_1 h3 =>
-        injection (Eq.symm h)
-        simp_all_arith[GetElem.getElem, List.get]
-      case cons.false.h_2 => contradiction
+    unfold findIdx? at h
+    split at h
+    next h => injection h.symm; simp_all_arith[Zero.zero]
+    next =>
+      rw [length_cons, Nat.succ_add]
+      have final := ih h
+      rw [Nat.add_succ] at final
+      assumption
+
+theorem findIdx?_bounds (h : findIdx? p xs = some idx) : idx < xs.length := findIdx?_bounds' h
+
+theorem findIdx?_prop_idx (h : findIdx? p xs s = some idx) : idx - s < length xs := by
+  have h1 := findIdx?_bounds' h
+  have h2 := findIdx?_lower_bound h
+  rw [←Nat.add_sub_cancel (length xs) s]
+  exact tsub_lt_tsub_right_of_le h2 h1
+
+theorem findIdx?_prop (h : findIdx? p xs s = some idx) : p (getElem xs (idx - s) (findIdx?_prop_idx h)) := by
+  induction xs generalizing idx s with
+  | nil => contradiction
+  | cons x xs ih =>
+    unfold findIdx? at h
+    split at h
+    next h => injection h.symm; simp_all[get]
+    next =>
+      have : idx ≠ 0 := by
+        intro falso
+        have : s + 1 ≤ idx := findIdx?_lower_bound h
+        cases this <;> contradiction
+      cases idx with
+      | zero => contradiction
+      | succ idx =>
+        have t := ih h
+        have : idx + 1 - s = (idx - s) + 1 := by
+          rw [Nat.add_comm]
+          rw [Nat.add_sub_assoc]
+          rw [Nat.add_comm]
+          apply Nat.le_of_succ_le_succ
+          exact findIdx?_lower_bound h
+        simp at t
+        simp [get, this, t]
 
 end List
 
@@ -51,59 +72,52 @@ namespace Cube.Simple
 
 inductive Ty where
 | nat
-| fun (x : Ty) (res : Ty)
+| fun (pre : Ty) (image : Ty)
 deriving Repr, DecidableEq
 
 inductive Ast where
-| var (x : String)
-| const (x : String)
-| lam (x : String) (ty : Ty) (b : Ast)
-| app (f : Ast) (x : Ast)
+| var (name : String)
+| const (name : String)
+| lam (var : String) (ty : Ty) (body : Ast)
+| app (func : Ast) (arg : Ast)
 
 inductive Expr where
 | bvar (idx : Nat)
 | fvar (name : String)
 | lam (ty : Ty) (body : Expr) (orig : String)
 | const (name : String)
-| app (f : Expr) (x : Expr)
+| app (func : Expr) (arg : Expr)
 deriving Repr, DecidableEq
 
 abbrev TranslationEnv := List String
 
-namespace TranslationEnv
-
-inductive Wf : TranslationEnv → Prop
-
-end TranslationEnv
-
 def Ast.toExpr : Ast → TranslationEnv → Expr
-| var x, vs =>
-  match vs.findIdx? (x = ·) with
+| var name, vs =>
+  match vs.findIdx? (name = ·) with
   | some idx => .bvar idx
-  | none => .fvar x
-| const x, _ => .const x
-| app f x, vs => .app (toExpr f vs) (toExpr x vs)
-| lam x ty b, vs => .lam ty (toExpr b <| x :: vs) x
+  | none => .fvar name
+| const name, _ => .const name
+| app func arg, vs => .app (toExpr func vs) (toExpr arg vs)
+| lam x ty body, vs => .lam ty (toExpr body <| x :: vs) x
 
 def Expr.toAst : Expr → TranslationEnv → Option Ast
 | bvar idx, vs => do
   let x ← vs[idx]?
   return .var x
-| fvar x, _ => some <| .var x
-| lam ty b x, vs => do
-    let body ← toAst b <| x :: vs
-    return .lam x ty body
+| fvar name, _ => some <| .var name
+| lam ty body name, vs => do
+    let body ← toAst body <| name :: vs
+    return .lam name ty body
 | const name, _ => some <| .const name
-| .app f x, vs => do
-    let fAst ← toAst f vs
-    let xAst ← toAst x vs
-    return .app fAst xAst
-
+| .app func arg, vs => do
+    let funcAst ← toAst func vs
+    let argAst ← toAst arg vs
+    return .app funcAst argAst
 
 declare_syntax_cat stlc
 declare_syntax_cat stlcTy
 syntax "ℕ" : stlcTy
-syntax stlcTy "->" stlcTy : stlcTy
+syntax stlcTy "→" stlcTy : stlcTy
 syntax "(" stlcTy ")" : stlcTy
 
 syntax ident : stlc
@@ -117,7 +131,7 @@ syntax "[stlc|" stlc "]" : term
 
 macro_rules
   | `([stlcTy| ℕ]) => `(Ty.nat)
-  | `([stlcTy| $a -> $b]) => `(Ty.fun [stlcTy| $a] [stlcTy| $b])
+  | `([stlcTy| $a → $b]) => `(Ty.fun [stlcTy| $a] [stlcTy| $b])
   | `([stlcTy| ($x)]) => `([stlcTy| $x])
 
   | `([stlcA| $x:ident]) =>
@@ -129,7 +143,6 @@ macro_rules
   | `([stlcA| λ $x : $ty . $b]) => `(Ast.lam $(quote x.getId.toString) [stlcTy| $ty]  [stlcA| $b])
   | `([stlcA| $f $x]) => `(Ast.app [stlcA| $f] [stlcA| $x])
   | `([stlcA| ($x)]) => `([stlcA| $x])
-
   | `([stlc| $t ]) => `(Ast.toExpr [stlcA| $t] [])
 
 theorem Ast.toExpr_inv_toAst (a : Ast) (xs : List String) : Expr.toAst (Ast.toExpr a xs) xs = some a := by
@@ -137,55 +150,171 @@ theorem Ast.toExpr_inv_toAst (a : Ast) (xs : List String) : Expr.toAst (Ast.toEx
   | var name =>
     simp only [Ast.toExpr]
     split
-    -- bvar case
     case var.h_1 idx h =>
-      -- unfold do notation
-      simp only [Expr.toAst,Bind.bind, Option.bind, Pure.pure] 
+      simp only [Expr.toAst,Bind.bind, Option.bind, Pure.pure]
       have h2 := List.findIdx?_bounds h
-      simp only [getElem?, h2, congrArg] -- TODO: possibly nicer
-      repeat (apply congrArg) -- TODO: replace with simp
+      simp only [getElem?, h2, congrArg, List.getElem_eq_get, Option.some.injEq, var.injEq]
       have h3 := List.findIdx?_prop h
       simp [of_decide_eq_true h3]
-    -- fvar case
     case var.h_2 => simp [Expr.toAst]
-  | const x => simp[Expr.toAst, Ast.toExpr]
-  | lam x ty b ih =>
-    simp[Expr.toAst, Ast.toExpr, Bind.bind, Option.bind, Pure.pure, ih] 
-  | app f x fih xih =>
-    simp[Expr.toAst, Ast.toExpr, Bind.bind, Option.bind, fih, xih, Pure.pure] 
-  
+  | const name => simp[Expr.toAst, Ast.toExpr]
+  | lam var ty body ih =>
+    simp[Expr.toAst, Ast.toExpr, Bind.bind, Option.bind, Pure.pure, ih]
+  | app func arg fih xih =>
+    simp[Expr.toAst, Ast.toExpr, Bind.bind, Option.bind, fih, xih, Pure.pure]
 
 theorem Ast.macro_correct (a : Ast) : Expr.toAst (Ast.toExpr a []) [] = some a := toExpr_inv_toAst a []
 
-#eval [stlc| λ x : ℕ . (λ y : ℕ -> ℕ . freee y x)]
+#eval [stlc| λ x : ℕ . (λ y : ℕ → ℕ . freee y x)]
 
 namespace Expr
 
 inductive ClosedTo : Nat → Expr → Prop where
-| bvar (h : n < m): ClosedTo m (.bvar n)
-| lam (h : ClosedTo (n + 1) body) : ClosedTo n (.lam ty body orig)
-| const : ClosedTo n (.const name)
-| app (h1 : ClosedTo n f) (h2 : ClosedTo n x) : ClosedTo n (.app f x)
+| bvar (idx m : Nat) (closed : idx < m): ClosedTo m (.bvar idx)
+| lam (closed : ClosedTo (n + 1) body) : ClosedTo n (.lam ty body orig)
+| const (n : Nat) (name : String) : ClosedTo n (.const name)
+| app (func arg : Expr) (closedFunc : ClosedTo n func) (closedArg : ClosedTo n arg) : ClosedTo n (.app func arg)
 
-abbrev Closed (e : Expr) := ClosedTo 0 e
+abbrev Closed (expr : Expr) := ClosedTo 0 expr
 
-def ClosedExpr := { e : Expr // Closed e }
+def ClosedExpr := { expr : Expr // Closed expr }
 
 abbrev Context := List Ty
 abbrev Env := String → Option Ty
 
-inductive Typing : Env → Context → Expr → Ty → Prop where
-| const (h : env name = some typ) : Typing env ctx (.const name) typ
-| app (h1 : Typing env ctx f (.fun t1 t2)) (h2 : Typing env ctx x t1) : Typing env ctx (.app f x) t2
-| lam (h : Typing env (t1 :: ctx) body t2) : Typing env ctx (.lam t1 body orig) (.fun t1 t2)
-| bvar (h : idx < ctx.length) : Typing env ctx (.bvar idx) (ctx.get ⟨idx, h⟩)
+def Context.set (ctx : Context) (n : Nat) (ty : Ty) : Context :=
+  match ctx, n with
+  | [], 0 => [ty]
+  | [], _ + 1 => []
+  | _ :: xs, 0 => ty :: xs
+  | x :: xs, n + 1 => x :: set xs n ty
 
-notation Δ " :: " Γ " ⊢ " e " : " t => Typing Δ Γ e t
+@[simp]
+theorem Context.set_nil_zero : Context.set [] 0 ty = [ty] := rfl
+
+@[simp]
+theorem Context.set_nil_succ : Context.set [] (i + 1) ty = [] := rfl
+
+@[simp]
+theorem Context.set_cons_zero : Context.set (x :: xs) 0 ty = ty :: xs := rfl
+
+@[simp]
+theorem Context.set_cons_succ : Context.set (x :: xs) (i + 1) ty = x :: (Context.set xs i ty) := rfl
+
+theorem Context.get_set (ctx : Context) (i : Nat) (h : i < (Context.set ctx i ty).length) : List.get (Context.set ctx i ty) ⟨i, h⟩ = ty :=
+  match ctx, i with
+  | [], 0 => rfl
+  | [], _ + 1 => by simp_arith [set, List.length] at h
+  | _ :: xs, 0 => rfl
+  | x :: xs, n + 1 => by
+    simp only [set]
+    apply get_set
+
+theorem Context.length_le_set_length : ctx.length ≤ (Context.set ctx i ty).length :=
+  match ctx, i with
+  | [], 0 => by simp_arith
+  | [], _ + 1 => by simp_arith
+  | _ :: xs, 0 => by simp_arith[set_cons_zero]
+  | x :: xs, n + 1 => by
+    simp only [Context.set_cons_succ, List.length_cons]
+    apply Nat.succ_le_succ
+    apply length_le_set_length
+
+theorem Context.set_bounds_eq_length (h : i < ctx.length) : (Context.set ctx i ty).length = ctx.length :=
+  match ctx, i with
+  | [], 0 => by contradiction
+  | [], _ + 1 => by contradiction
+  | _ :: xs, 0 => by simp
+  | x :: xs, n + 1 => by
+    simp only [set_cons_succ, List.length_cons, Nat.succ.injEq]
+    apply set_bounds_eq_length
+    apply Nat.lt_of_succ_lt_succ
+    assumption
+
+theorem Context.set_out_of_bounds_eq_length (h : ctx.length < i) : (Context.set ctx i ty).length = ctx.length :=
+  match ctx, i with
+  | [], 0 => by contradiction
+  | [], _ + 1 => by simp
+  | _ :: xs, 0 => by simp
+  | x :: xs, n + 1 => by
+    simp only [set_cons_succ, List.length_cons, Nat.succ.injEq]
+    apply set_out_of_bounds_eq_length
+    apply Nat.lt_of_succ_lt_succ
+    assumption
+
+theorem Context.set_succ_bound_eq_append (h : i = ctx.length) : (Context.set ctx i ty) = ctx ++ [ty] :=
+  match ctx, i with
+  | [], 0 => by simp
+  | [], _ + 1 => by contradiction
+  | _ :: xs, 0 => by contradiction
+  | x :: xs, n + 1 => by
+    simp [set_cons_succ, List.length_cons, Nat.succ.injEq, true_and]
+    apply set_succ_bound_eq_append
+    injection h
+
+theorem Context.set_succ_bound_length_eq_succ_length (h : i = ctx.length) : (Context.set ctx i ty).length = ctx.length + 1 := by
+  simp_all[Context.set_succ_bound_eq_append]
+
+theorem Context.get_set_neq (h1 : i = ctx.length) (h2 : idx ≠ i) (h3 : idx < List.length ctx) : List.get (Context.set ctx i ty) ⟨idx, by rw[Context.set_succ_bound_length_eq_succ_length]; apply Nat.lt_succ_of_lt h3; exact h1⟩ = List.get ctx ⟨idx, h3⟩ :=
+  match ctx, i with
+  | [], 0 => by contradiction
+  | [], _ + 1 => by contradiction
+  | _ :: xs, 0 => by contradiction
+  | x :: xs, n + 1 => by
+    simp only [set_cons_succ, List.length_cons]
+    cases idx with
+    | zero => simp
+    | succ idx =>
+      simp only [List.get_cons_succ]
+      apply get_set_neq
+      injection h1
+      next =>
+        intro h
+        apply h2
+        simp [h]
+
+theorem Context.get_set_irrelevant (ctx : Context) (i1 i2 : Nat) (h1 : i2 < ctx.length) (h2 : i1 ≠ i2) : List.get (Context.set ctx i1 ty) ⟨i2, Nat.lt_of_lt_of_le h1 length_le_set_length⟩ = List.get ctx ⟨i2, h1⟩ :=
+  match ctx, i1 with
+  | [], 0 => by
+    simp only [set, List.length] at h1
+    cases h1
+    repeat contradiction
+  | [], _ + 1 => by simp [Context.set_nil_succ]
+  | _ :: xs, 0 => by
+    simp only [Context.set_cons_zero]
+    cases i2 with
+    | zero => contradiction
+    | succ i2 => simp only [List.get_cons_succ]
+  | x :: xs, n + 1 => by
+    simp only [Context.set_cons_succ]
+    cases i2 with
+    | zero => simp
+    | succ i2 =>
+      simp only [List.get_cons_succ]
+      apply get_set_irrelevant
+      simp_all
+
+inductive Typing : Env → Context → Expr → Ty → Prop where
+| const (in_env : env name = some typ) : Typing env ctx (.const name) typ
+| app (func_type : Typing env ctx func (.fun t1 t2)) (arg_type : Typing env ctx arg t1) : Typing env ctx (.app func arg) t2
+| lam (body_type : Typing env (t1 :: ctx) body t2) : Typing env ctx (.lam t1 body orig) (.fun t1 t2)
+| bvar (idx : Nat) (bound : idx < ctx.length) : Typing env ctx (.bvar idx) (ctx.get ⟨idx, bound⟩)
+
+notation:40 "("Δ ", " Γ ")" " ⊢ " e " : " t => Typing Δ Γ e t
+
+theorem ClosedTo.of_typed (h : (env, ctx) ⊢ expr : ty) : ClosedTo ctx.length expr := by
+  induction h with
+  | const => apply ClosedTo.const
+  | app _ _ func_ih arg_ih => simp [ClosedTo.app, *]
+  | bvar => simp [ClosedTo.bvar, *]
+  | lam =>
+    apply ClosedTo.lam
+    assumption
 
 def ClosedExpr.infer (expr : ClosedExpr) (env : Env) : Option Ty :=
   go expr.val expr.property [] rfl
 where
-  go {n : Nat} (expr : Expr) (h1 : ClosedTo n expr) (ctx : Context) (h2 : ctx.length = n) : Option Ty := 
+  go {n : Nat} (expr : Expr) (h1 : ClosedTo n expr) (ctx : Context) (h2 : ctx.length = n) : Option Ty :=
     match expr with
     | .bvar idx =>
       if hVar:idx < n then
@@ -217,35 +346,31 @@ where
       | some ty => some ty
       | none => none
 
-theorem ClosedExpr.infer.go_sound (expr : Expr) (env : Env) (ctx : Context) (h1 : ClosedTo ctx.length expr) (h2 : ClosedExpr.infer.go env expr h1 ctx rfl = some t) : env :: ctx ⊢ expr : t := by
+theorem ClosedExpr.infer.go_sound (expr : Expr) (env : Env) (ctx : Context) (h1 : ClosedTo ctx.length expr) (h2 : ClosedExpr.infer.go env expr h1 ctx rfl = some t) : (env, ctx) ⊢ expr : t := by
   induction expr generalizing t ctx with
   | fvar => contradiction
   | const name =>
     unfold infer.go at h2
-    split at h2
-    next =>
-      apply Typing.const
-      simp [*]
-    next => contradiction
+    split at h2 <;> simp [Typing.const, *]
   | app f x fih xih =>
-    simp [infer.go, Id.run] at h2
+    simp only [infer.go, Id.run] at h2
     repeat split at h2
     next =>
       injections
       simp_all
       apply Typing.app
-      case h1 =>
+      case func_type =>
         apply fih _ (by cases h1; assumption)
         assumption
-      case h2 =>
+      case arg_type =>
         apply xih _ (by cases h1; assumption)
         assumption
     repeat contradiction
   | lam ty body _ ih =>
-    simp [infer.go] at h2
+    simp only [infer.go] at h2
     split at h2
     next _ _ t3 h3 =>
-      simp at h2
+      injections h2
       rw[←h2]
       apply Typing.lam
       apply ih
@@ -254,52 +379,32 @@ theorem ClosedExpr.infer.go_sound (expr : Expr) (env : Env) (ctx : Context) (h1 
   | bvar idx =>
     have idx_get : t = ctx.get ⟨idx, (by cases h1; assumption)⟩ := by
       unfold go at h2
-      split at h2
-      next =>
-        injections
-        simp [*]
-      next => contradiction
+      split at h2 <;> simp_all
     rw[idx_get]
     apply Typing.bvar
 
-theorem ClosedExpr.infer_sound (expr : ClosedExpr) (env : Env) (h : expr.infer env = some t) : env :: [] ⊢ expr.val : t := by
+theorem ClosedExpr.infer_sound (expr : ClosedExpr) (env : Env) (h : expr.infer env = some t) : (env, []) ⊢ expr.val : t := by
   unfold infer at h
   apply ClosedExpr.infer.go_sound
   assumption
 
-theorem ClosedExpr.infer.go_complete (expr : Expr) (env : Env) (ctx : Context) (h1 : ClosedTo ctx.length expr) (h2 : env :: ctx ⊢ expr : t) : ClosedExpr.infer.go env expr h1 ctx rfl = some t := by
+theorem ClosedExpr.infer.go_complete (expr : Expr) (env : Env) (ctx : Context) (h1 : ClosedTo ctx.length expr) (h2 : (env, ctx) ⊢ expr : t) : ClosedExpr.infer.go env expr h1 ctx rfl = some t := by
   induction h2 with
   | const =>
     unfold go
-    split
-    next => simp_all
-    next => simp_all
-  | app hf hx ih1 ih2 =>
+    split <;> simp_all
+  | app _ _ ih1 ih2 =>
     have ih1 := ih1 (by cases h1; assumption)
     have ih2 := ih2 (by cases h1; assumption)
     simp[go, Id.run]
-    repeat split
-    next => simp_all
-    next => simp_all
-    next _ _ _ t _ _ _ _ _ _ _ _ _ h =>
-      apply False.elim
-      apply h t
-      assumption
-    next _ _ _ t1 t2 _ _ _ _ h =>
-      apply False.elim
-      apply h t1 t2
-      assumption
+    repeat split <;> simp_all
   | lam _ ih =>
     have ih := ih (by cases h1; assumption)
     simp[go]
-    split
-    next => simp_all
-    next _ _ _ _ _ _ _ h =>
-      apply False.elim
-      apply h _ ih
+    split <;> simp_all
   | bvar h_idx => simp_all[go]
 
-theorem ClosedExpr.infer_complete (expr : ClosedExpr) (env : Env) (h : env :: [] ⊢ expr.val : t) :  expr.infer env = some t := by
+theorem ClosedExpr.infer_complete (expr : ClosedExpr) (env : Env) (h : (env, []) ⊢ expr.val : t) :  expr.infer env = some t := by
   unfold infer
   apply ClosedExpr.infer.go_complete _ _ []
   assumption
@@ -310,7 +415,7 @@ def ClosedExpr.typecheck (env : Env) (expr : ClosedExpr) (typ : Ty) : Bool := Id
       return true
   return false
 
-theorem ClosedExpr.typecheck_sound (expr : ClosedExpr) (t : Ty) (env : Env) (h : expr.typecheck env t = true) : env :: [] ⊢ expr.val : t := by
+theorem ClosedExpr.typecheck_sound (expr : ClosedExpr) (t : Ty) (env : Env) (h : expr.typecheck env t = true) : (env, []) ⊢ expr.val : t := by
   simp [typecheck, Id.run] at h
   repeat split at h
   next =>
@@ -318,7 +423,7 @@ theorem ClosedExpr.typecheck_sound (expr : ClosedExpr) (t : Ty) (env : Env) (h :
     simp [*]
   repeat contradiction
 
-theorem ClosedExpr.typecheck_complete (expr : ClosedExpr) (t : Ty) (env : Env) (h : env :: [] ⊢ expr.val : t) : expr.typecheck env t = true := by
+theorem ClosedExpr.typecheck_complete (expr : ClosedExpr) (t : Ty) (env : Env) (h : (env, []) ⊢ expr.val : t) : expr.typecheck env t = true := by
   simp [typecheck, Id.run]
   split
   next _ t2 h2 =>
@@ -333,7 +438,7 @@ theorem ClosedExpr.typecheck_complete (expr : ClosedExpr) (t : Ty) (env : Env) (
     apply infer_complete
     assumption
 
-theorem Typing.unique (h1 : env :: ctx ⊢ expr : ty1) (h2 : env :: ctx ⊢ expr : ty2) : ty1 = ty2 := by
+theorem Typing.unique (h1 : (env, ctx) ⊢ expr : ty1) (h2 : (env, ctx) ⊢ expr : ty2) : ty1 = ty2 := by
   match term:h1 with
   | .const .. => cases h2; simp_all
   | .bvar .. => cases h2; simp_all
@@ -348,38 +453,257 @@ theorem Typing.unique (h1 : env :: ctx ⊢ expr : ty1) (h2 : env :: ctx ⊢ expr
       have := unique h3 h4
       simp_all
 
-def abstract (target : String) (expr : Expr) : Expr :=
-  go 0 expr
-where
-  go (idx : Nat) (expr : Expr) :=
-    match expr with
-    | .fvar name =>
-      if target = name then
-        .bvar idx
-      else
-        .fvar name
-    | .app fn arg => .app (go idx fn) (go idx arg)
-    | .lam ty body orig => .lam ty (go (idx + 1) body) orig
-    | .const name => .const name
-    | .bvar idx => .bvar idx
+theorem Typing.weakening (h1 : ctx' = ctx ++ additional) (h2 : (env, ctx) ⊢ expr : typ) : (env, ctx') ⊢ expr : typ := by
+  induction h2 generalizing ctx' with
+  | const =>
+    apply Typing.const
+    assumption
+  | app _ _ ihf ihx =>
+    apply Typing.app
+    case func_type =>
+      apply ihf
+      assumption
+    case arg_type =>
+      apply ihx
+      assumption
+  | lam _ ih =>
+    apply Typing.lam
+    apply ih
+    simp[h1]
+  | bvar idx =>
+    rw[h1, ←List.get_append idx]
+    apply Typing.bvar
 
-def instantiate (image : Expr) (expr : Expr) : Expr :=
-  go 0 expr
-where
-  go (targetIdx : Nat) (expr : Expr) :=
-    match expr with
-    | .bvar idx =>
-      if idx = targetIdx then
-        image
-      else
-        .bvar idx
-    | .app fn arg => .app (go targetIdx fn) (go targetIdx arg)
-    | .lam ty body orig => .lam ty (go (targetIdx + 1) body) orig
-    | .fvar name => .fvar name
-    | .const name => .const name
+theorem Typing.weakening_empty (ctx : Context) (h : (env, []) ⊢ expr : typ) : (env, ctx) ⊢ expr : typ :=
+  Typing.weakening (List.nil_append ctx).symm h
+
+-- From I'm not a number I'm a free variable
+def abstract (target : String) (expr : Expr) (idx : Nat := 0): Expr :=
+  match expr with
+  | .fvar name =>
+    if target = name then
+      .bvar idx
+    else
+      .fvar name
+  | .app fn arg => .app (abstract target fn idx) (abstract target arg idx )
+  | .lam ty body orig => .lam ty (abstract target body (idx + 1)) orig
+  | .const name => .const name
+  | .bvar idx => .bvar idx
+
+def instantiate (image : Expr) (expr : Expr) (targetIdx : Nat := 0): Expr :=
+  match expr with
+  | .bvar idx =>
+    if idx = targetIdx then
+      image
+    else
+      .bvar idx
+  | .app fn arg => .app (instantiate image fn targetIdx ) (instantiate image arg targetIdx )
+  | .lam ty body orig => .lam ty (instantiate image body (targetIdx + 1)) orig
+  | .fvar name => .fvar name
+  | .const name => .const name
 
 def substitute (image : Expr) (name : String) (expr : Expr) : Expr :=
   expr.abstract name |>.instantiate image
+
+theorem Typing.instantiate_preserves (h1 : (env, []) ⊢ v : ty) (h2 : (env, (Context.set ctx i ty)) ⊢ expr : ty') : (env, ctx) ⊢ (instantiate v expr i) : ty' := by
+  induction expr generalizing ctx ty' i with
+  | const =>
+    simp only [instantiate]
+    cases h2
+    apply Typing.const
+    assumption
+  | bvar idx =>
+    simp only [instantiate]
+    split
+    case inl h =>
+      have : ty' = ty := by
+        rw[h] at h2
+        cases h2
+        apply Context.get_set
+      apply weakening_empty
+      rw[this]
+      assumption
+    case inr neq =>
+      cases h2 with
+      | bvar _ bound  =>
+        cases Nat.lt_trichotomy i ctx.length with
+        | inl h =>
+          have neq_symm : i ≠ idx := by intro h; apply neq h.symm
+          have lt : idx < ctx.length := by
+            simp only [Context.set_bounds_eq_length, h] at bound
+            assumption
+          simp [Context.get_set_irrelevant, lt, neq_symm, Typing.bvar]
+        | inr h =>
+          cases h with
+          | inl =>
+            rw [Context.set_succ_bound_length_eq_succ_length] at bound
+
+            have helper {n m : Nat} (h1 : n < m + 1) (h2 : n ≠ m) : n < m := by
+              cases lt_or_gt_of_ne h2 <;> linarith
+            have : idx < List.length ctx := helper (by assumption) (by simp_all)
+            next =>
+              rw [Context.get_set_neq]
+              apply Typing.bvar
+              assumption
+              next => intro h; apply neq h
+              assumption
+            next => assumption
+          | inr =>
+            rw [Context.get_set_irrelevant]
+            next => apply Typing.bvar
+            next =>
+              rw [Context.set_out_of_bounds_eq_length] at bound
+              repeat assumption
+            next => intro h; apply neq h.symm
+  | fvar => cases h2
+  | lam _ _ _ ih =>
+    simp only [instantiate]
+    cases h2
+    apply Typing.lam
+    apply ih
+    assumption
+  | app _ _ fih xih =>
+    simp only [instantiate]
+    cases h2
+    apply Typing.app
+    case func_type =>
+      apply fih
+      repeat assumption
+    case arg_type =>
+      apply xih
+      repeat assumption
+
+@[simp]
+def isLam : Expr → Bool
+| .lam .. => true
+| _ => false
+
+inductive Value : Expr → Prop where
+| lam : Value (.lam ty body orig)
+| const : Value (.const name)
+| constApp (h : Value v) : Value (.app (.const name) v)
+| app (h1 : Value f) (h2 : ¬f.isLam) (h3 : Value v) : Value (.app f v)
+
+inductive BetaStep : Expr → Expr → Prop where
+| lamApp : BetaStep (.app (.lam ty body orig) arg) (instantiate arg body)
+| leftApp (h : BetaStep t1 t1') : BetaStep (.app t1 t2) (.app t1' t2)
+| rightApp (h1 : Value t1) (h2 : BetaStep t2 t2') : BetaStep (.app t1 t2) (.app t1 t2')
+
+inductive Multi (R : α → α → Prop) : α → α → Prop where
+| rfl : Multi R x x
+| step (x y z : α) (h1 : R x y) (h2 : Multi R y z) : Multi R x z
+
+def normal_form (R : α → α → Prop) (t : α) : Prop := ¬ ∃ t', R t t'
+def step_normal_form (expr : Expr) : Prop := normal_form BetaStep expr
+abbrev BetaReduction := Multi BetaStep
+
+notation t1 " →β " t2 => BetaStep t1 t2
+notation t1 " →β* " t2 => BetaReduction t1 t2
+
+example : [stlc| (λ x : ℕ → ℕ . x) (λ x : ℕ . x)] →β [stlc| (λ x : ℕ . x)] := by
+  simp [Ast.toExpr, List.findIdx?]
+  apply BetaStep.lamApp
+
+theorem Expr.subject_reduction (expr : Expr) (typed_expr : (env, []) ⊢ expr : ty) (reduces : expr →β expr') : (env, []) ⊢ expr' : ty := by
+  cases typed_expr with
+  | const => cases reduces
+  | app =>
+    cases reduces
+    case lamApp lam_typed =>
+      cases lam_typed with
+      | lam body_typed =>
+        rw [←Context.set_nil_zero] at body_typed
+        apply Typing.instantiate_preserves
+        repeat assumption
+    case leftApp =>
+      apply Typing.app
+      apply subject_reduction
+      repeat assumption
+    case rightApp =>
+      apply Typing.app
+      assumption
+      apply subject_reduction
+      repeat assumption
+  | lam => cases reduces
+  | bvar => cases reduces
+
+theorem Value.normal (expr : Expr) (h : Value expr) : step_normal_form expr := by
+  induction h with
+  | lam =>
+    intro h
+    cases h with
+    | intro t' ht' =>
+      cases ht'
+  | const =>
+    intro h
+    cases h with
+    | intro t' ht' =>
+      cases ht'
+  | constApp _ ih =>
+    intro h
+    cases h with
+    | intro t' ht' =>
+      cases ht' with
+      | leftApp h => cases h
+      | rightApp h =>
+        apply False.elim
+        apply ih
+        constructor
+        assumption
+  | app h1 h2 _ h4 h5 =>
+    intro h
+    cases h with
+    | intro t' ht' =>
+      cases ht' with
+      | lamApp => simp[isLam] at h2
+      | leftApp =>
+        apply h4
+        constructor
+        assumption
+      | rightApp =>
+        apply h5
+        constructor
+        assumption
+
+theorem Value.terminated (expr expr' : Expr) (h1 : Value expr) (h2 : expr →β* expr') : expr = expr' := by
+  cases h2 with
+  | rfl => rfl
+  | step =>
+    apply False.elim
+    apply Value.normal
+    assumption
+    constructor
+    assumption
+
+def halts (expr : Expr) : Prop := ∃ expr', (expr →β expr') ∧ Value expr'
+
+def R (t : Ty) (expr : Expr) : Prop :=
+  (∀ env, (env , []) ⊢ expr : t) ∧ halts expr ∧ match t with
+  | .nat => True
+  | .fun t1 t2 => ∀ s, R t1 s → R t2 (.app expr s)
+
+theorem R.halts (h : R typ expr) : halts expr := by
+  cases typ <;> (
+    unfold R at h
+    cases h with
+    | intro left right =>
+      cases right;
+      assumption
+  )
+
+theorem R.typable (h : R typ expr) (env : Env) : (env, []) ⊢ expr : typ := by
+  cases typ <;> (
+    unfold R at h;
+    cases h with
+    | intro left right => exact left env)
+
+
+theorem R.beta_reduction_preserves (h1 : expr →β expr') (h2 : R typ expr) : R typ expr' := by
+  sorry
+
+theorem Expr.strong_normalization (expr : Expr) (typed : (env, ctx) ⊢ expr : ty) : ∃ target, (expr →β target) ∧ Value target := by
+  sorry
+
 end Expr
 
 end Cube.Simple
