lakefile.lean
@@ -5,6 +5,8 @@ package cube {
   -- add package configuration options here
 }
 
+require mathlib from git "https://github.com/leanprover-community/mathlib4" @ "master"
+
 @[default_target]
 lean_lib Cube {
   -- add library configuration options here
